Rework definition of `iHandler`s laying the groundwork so that `EFork` can be treated correctly (currently, post-conditions are duplicated).

src/handler.v
@@ -1,55 +1,69 @@
 From iris.proofmode Require Import proofmode.
 From iris.base_logic.lib Require Import iprop.
 From ITree Require Import ITree.
+From ITree Require Import Eq.
+From ITree Require Import TranslateFacts.
+From iris.itree Require Import event.
 
 (** An [iHandler] is the used-specified "recipe" used to define a custom
 weakest [WPi]. It specifies how to interpret an event logically, given weakest
 preconditions for continuations of the itree.
-
-An [iHandler] is a function that takes an event [E A] with answer type [A],
-as well as continuations [k : A → iProp Σ], and produces a new logical
-expression [iProp Σ]. Given an itree [Vis e t], [ihandle e k] should be
-thought of as a verification condition for this itree, assuming that
-[k a : iProp Σ] is a verification condition for the itree [t a]. We refer
-the reader to [WPi] for a precise meaning of this intuition.
 *)
-Record iHandler Σ (E : Type → Type) := IHandler {
-  ihandle : ∀ A, E A → (A → iProp Σ) → iProp Σ;
+Record iHandler Σ (EF : (Type → Type) → Type → Type) := IHandler {
+  ihandle :> ∀ preE A,
+      (* Event [e] *)
+      EF preE A
+      (* Continuation conditions [λ a, ▷ WPi k a @ H; ∅ {{ Φ }}] *)
+    → (A → iProp Σ)
+      (* Conditions for spawning threads [λ a, ▷ WPi t @ H; ⊤ {{ True }}] *)
+    → (itree preE unit → iProp Σ)
+      (* Condition [WPi Vis e k @ H; M {{ Φ }}] *)
+    → iProp Σ;
 }.
 Arguments IHandler {_ _} _.
-Coercion ihandle : iHandler >-> Funclass.
 
 Import EqNotations.
 (** Convenient helper for constructing [iHandler]s that treat only events with
-a particular, fixed answrer tytpe [A]. *)
-Definition IHandlerT {Σ} {E : Type → Type} {A : Type}
-  (H : (E A → (A → iProp Σ) → iProp Σ)) : iHandler Σ E :=
-  IHandler (λ A' e Φ, ∃ x : A' = A, H
-    (rew [λ A, E A] x in e)
-    (rew [λ A, (A → iProp Σ)%type] x in Φ))%I.
+a particular, fixed answrer type [A]. *)
+Definition IHandlerT {Σ} {EF : (Type → Type) → Type → Type} {A : Type}
+  (H : ∀ preE, (EF preE A → (A → iProp Σ) → (itree preE unit → iProp Σ) → iProp Σ)) :
+  iHandler Σ EF :=
+  IHandler (λ preE A' e Φ s, ∃ x : A' = A, H preE
+    (rew [λ A, EF preE A] x in e)
+    (rew [λ A, (A → iProp Σ)%type] x in Φ)
+    s)%I.
 
 (** Restricts a handler along a morphism of event types. *)
-Definition restrictH {Σ E2} E1 (H1 : iHandler Σ E2) `{!E1 -< E2} : iHandler Σ E1 :=
-  IHandler (λ A e Φ, H1 A (subevent A e) Φ)%I.
+Definition restrictH {Σ EF2} EF1 (H1 : iHandler Σ EF2) `{EF1 --< EF2} : iHandler Σ EF1 :=
+  IHandler (λ preE A e Φ s, H1 preE A (subevent A e) Φ s)%I.
 
 (** Asserts that the [iHandler] [H1] is stronger than [H2]. *)
-Definition subH {Σ E} (H1 H2 : iHandler Σ E) : iProp Σ :=
-  ∀ T e Φ, H1 T e Φ -∗ H2 T e Φ.
+Definition subH {Σ EF} (H1 H2 : iHandler Σ EF) : iProp Σ :=
+  ∀ preE A e Φ s, H1 preE A e Φ s -∗ H2 preE A e Φ s.
+
+Lemma subH_transitive {Σ EF} (H1 H2 H3 : iHandler Σ EF) :
+  subH H1 H2 -∗
+  subH H2 H3 -∗
+  subH H1 H3.
+Proof.
+  iIntros "Hsub1 Hsub2" (preE A e Φ s) "HH1". iApply "Hsub2". by iApply "Hsub1".
+Qed.
+
 (** [inH H1 H2] means that, on events [E1], [H1] is stronger than [H2]. *)
-Class inH {Σ E1 E2} `{!E1 -< E2} (H1 : iHandler Σ E1) (H2 : iHandler Σ E2) :=
-  is_inH : ⊢ subH H1 (restrictH E1 H2).
+Class inH {Σ EF1 EF2} `{f : EF1 --< EF2} (H1 : iHandler Σ EF1) (H2 : iHandler Σ EF2) :=
+  is_inH : ⊢ subH H1 (restrictH EF1 H2).
 
 (** Disjunction of two [iHandler]s. *)
 Global Instance iHandler_union Σ E : Union (iHandler Σ E) :=
-  λ H1 H2, IHandler (λ T e Φ, H1 T e Φ ∨ H2 T e Φ)%I.
+  λ H1 H2, IHandler (λ preE A e Φ s, H1 preE A e Φ s ∨ H2 preE A e Φ s)%I.
 
-Lemma subH_union_l Σ E H1 H2 :
-  ⊢ subH (Σ:=Σ) (E:=E) H1 (H1 ∪ H2).
-Proof. iIntros (???) "HH". by iLeft. Qed.
-Lemma subH_union_r Σ E H1 H2 :
-  ⊢ subH (Σ:=Σ) (E:=E) H2 (H1 ∪ H2).
-Proof. iIntros (???) "HH". by iRight. Qed.
-Global Instance in_union_l {Σ E} (H1 : iHandler Σ E) (H2 : iHandler Σ E) : inH H1 (H1 ∪ H2).
+Lemma subH_union_l Σ EF H1 H2 :
+  ⊢ subH (Σ:=Σ) (EF:=EF) H1 (H1 ∪ H2).
+Proof. iIntros (?????) "HH". by iLeft. Qed.
+Lemma subH_union_r Σ EF H1 H2 :
+  ⊢ subH (Σ:=Σ) (EF:=EF) H2 (H1 ∪ H2).
+Proof. iIntros (?????) "HH". by iRight. Qed.
+Global Instance in_union_l {Σ EF} (H1 : iHandler Σ EF) (H2 : iHandler Σ EF) : inH H1 (H1 ∪ H2).
 Proof. apply subH_union_l. Qed.
 Global Instance in_union_r {Σ E} (H1 : iHandler Σ E) (H2 : iHandler Σ E) : inH H2 (H1 ∪ H2).
 Proof. apply subH_union_r. Qed.
