src/wpi.v
@@ -4,9 +4,12 @@ From iris.base_logic.lib Require Import iprop.
 From iris.base_logic.lib Require Export ghost_var.
 From iris.base_logic.lib Require Export fancy_updates.
 From iris.itree Require Import handler.
+From iris.itree Require Import event.
 From ITree Require Import ITree.
+From ITree Require Import CategoryFunctor.
 From ITree Require Import Interp.InterpFacts.
 From ITree Require Import Eq.
+From ITree Require Import Eqit.
 
 (** Weaken a predicate transformer into a monotonic predicate transformer in a
 universal way. *)
@@ -65,30 +68,102 @@ Section bi_mono1.
   Qed.
 End bi_mono1.
 
-Section wp_itree.
-  Context {Σ : gFunctors} {E : Type → Type} {R : Type}.
-  Context `{!invGS_gen HasNoLc Σ}.
+(* A variant of [bi_mono1] which makes predicate transformer monotonic only
+under a persistency modality. *)
+Definition bi_mono1_pers {PROP : bi} {A} (P : (A → PROP) → PROP) : (A → PROP) → PROP :=
+  λ Q, (∃ Q', P Q' ∗ □ (∀ a, Q' a -∗ Q a))%I.
 
-  (** The definition of the weakest precondition, prior to taking the fixpoint. *)
-  Definition wpi_pre (H : iHandler Σ E)
-    (wp_itree : leibnizO (itree E R) -d> (leibnizO R -d> iPropO Σ) -d> iPropO Σ) :
-                leibnizO (itree E R) -d> (leibnizO R -d> iPropO Σ) -d> iPropO Σ :=
+Section bi_mono1_pers.
+  Context {PROP : bi} {A : Type}.
+  Implicit Types (P : (A → PROP) → PROP).
+
+  Lemma bi_mono1_pers_intro0 P Q :
+    P Q -∗
+    bi_mono1_pers P Q.
+  Proof. iIntros "?". iExists _. iFrame. iModIntro. iIntros (?) "$". Qed.
+
+  Lemma bi_mono1_pers_mono P Q1 Q2 :
+    □ (∀ x, Q1 x -∗ Q2 x) -∗
+    bi_mono1_pers P Q1 -∗
+    bi_mono1_pers P Q2.
+  Proof.
+    iIntros "#HQ [% [HP #HQ1]]". iExists _. iFrame "HP". iModIntro.
+    iIntros (?) "?". iApply "HQ". by iApply "HQ1".
+  Qed.
+
+  Lemma bi_mono1_pers_mono_l P1 P2 Q :
+    (∀ Q, P1 Q -∗ P2 Q) -∗
+    bi_mono1_pers P1 Q -∗
+    bi_mono1_pers P2 Q.
+  Proof.
+    iIntros "HQ [% [HP HQ1]]". iExists _. iFrame "HQ1". by iApply "HQ".
+  Qed.
+
+  Lemma bi_mono1_pers_elim P Q :
+    □ (∀ Q', (∀ x, Q' x -∗ Q x) -∗ P Q' -∗ P Q) -∗
+    bi_mono1_pers P Q -∗
+    P Q.
+  Proof. iIntros "#HP [% [?#?]]". iApply ("HP" with "[$] [$]"). Qed.
+
+  Lemma bi_mono1_pers_intro P Q Q' :
+    □ (∀ x, Q' x -∗ Q x) -∗
+    P Q' -∗
+    bi_mono1_pers P Q.
+  Proof.
+    iIntros "#HQ HP".
+    iApply (bi_mono1_pers_mono with "HQ [HP]").
+    by iApply bi_mono1_pers_intro0.
+  Qed.
+End bi_mono1_pers.
+
+Global Instance itree_equiv (E : Type → Type) R : Equiv (itree E R) := eq_itree (=).
+
+Global Instance eq_itree_iff {E R} (t' : itree E R) :
+  Proper (eq_itree (=) ==> iff) (λ t, t ≅ t').
+Proof.
+  intros t1 t2 Heqit. by rewrite Heqit.
+Qed.
+
+Section wp_itree.
+  Context {Σ : gFunctors} {R : Type} `{!EventFixpoint EF E} `{!invGS_gen HasNoLc Σ}.
+
+  Import EqNotations.
+
+  (** The definition of the weakest precondition, prior to taking the fixpoint.
+
+  The result is of type [option R]. [None] represents safe termination. This is
+  a workaround to avoid dependent typing while still allowing us to consider
+  in addition to [itree E R] also [itree E unit], which is needed for e.g.
+  spawning new threads. *)
+  Definition wpi_pre (H : iHandler Σ EF)
+    (wpi : discreteO (itree E (option R)) -d> (leibnizO R -d> iPropO Σ) -d> iPropO Σ) :
+           discreteO (itree E (option R)) -d> (leibnizO R -d> iPropO Σ) -d> iPropO Σ :=
     λ t Φ,
       (|={∅}=>
-        (∃ r, ⌜t ≅ Ret r⌝ ∗ Φ r) ∨
-        (∃ t', ⌜t ≅ Tau t'⌝ ∗ ▷ wp_itree t' Φ) ∨
-        (* To deal with the fact that [iHandler]s need not be monotonic, we
-        close [H] so as to make it monotonic. Without this, the weakest
-        precondition may fail to satisfy desirable properties such as the rule
-        of consequence. *)
-        (∃ T (e : E T) k, ⌜t ≅ Vis e k⌝ ∗ bi_mono1 (H T e) (λ x, ▷ wp_itree (k x) Φ))
+        (* Used to terminate forked threads. *)
+        (⌜t ≅ Ret None⌝ ∗ |={∅, ⊤}=> True) ∨
+        (∃ r, ⌜t ≅ Ret (Some r)⌝ ∗ Φ r) ∨
+        (∃ t', ⌜t ≅ Tau t'⌝ ∗ ▷ wpi t' Φ) ∨
+        (* To deal with the fact that [iHandler]s need not be monotonic in the
+        continuations, we close [H] so as to make it monotonic. Without this,
+        the weakest precondition may fail to satisfy desirable properties such
+        as the rule of consequence and the frame rule. *)
+        (∃ A (e : E A) k, ⌜t ≅ Vis e k⌝ ∗
+          bi_mono1
+            (λ f,
+              bi_mono1_pers
+                (λ g, H E A (rew [λ T, T A] eq_fix in e) f g)
+                (λ t', ▷ |={⊤, ∅}=> wpi (ITree.map (const None) t') (λ _, (* unreachable *) False))
+            )
+            (λ a, ▷ wpi (k a) Φ)
+        )
       )%I.
 
-  Global Instance wpi_pre_ne n H:
+  Global Instance wpi_pre_ne n H :
     Proper ((dist n ==> dist n ==> dist n) ==> dist n ==> dist n ==> dist n) (wpi_pre H).
   Proof.
-    move => ?? Hwp ?? -> ?? HΦ. rewrite /wpi_pre/bi_mono1.
-    repeat (f_equiv || eapply Hwp || eapply HΦ || reflexivity).
+    intros wp1 wp2 Hwp t1 t2 Ht Φ1 Φ2 HΦ. rewrite /wpi_pre/bi_mono1/bi_mono1_pers.
+    by repeat (apply eq_itree_iff || f_equiv || eapply Hwp).
   Qed.
 
   Lemma wpi_pre_mono H wp1 wp2:
@@ -96,15 +171,21 @@ Section wp_itree.
     → ∀ t Φ, wpi_pre H wp1 t Φ -∗ wpi_pre H wp2 t Φ.
   Proof.
     iIntros "#Hinner" (t Φ) "Hwp".
-    iMod "Hwp" as "[?|[[%t' [% ?]]|(%T&%e&%k&%&Hwp)]]"; iModIntro.
-    - iLeft. by iFrame.
-    - iRight. iLeft. iExists _. iSplit; [done|]. iModIntro. by iApply "Hinner".
-    - iRight. iRight. iExists _, _, _. iSplit; [done|].
-      iApply (bi_mono1_mono with "[] Hwp"). iIntros (?) "?". by iApply "Hinner".
+    iMod "Hwp" as "[[%Ht >_]|[?|[[%t' [% ?]]|(%A&%e&%k&%&Hwp)]]]".
+    - iLeft. iApply fupd_mask_intro; first done. iIntros "Hfupd".
+      iSplit; first done. by iMod "Hfupd".
+    - iModIntro. iRight. iLeft. by iFrame.
+    - iModIntro. iRight. iRight. iLeft. iExists _. iSplit; [done|]. iModIntro. by iApply "Hinner".
+    - iModIntro. iRight. iRight. iRight. iExists _, _, _. iSplit; [done|].
+      iApply bi_mono1_mono_l; [|iApply (bi_mono1_mono with "[] Hwp")].
+      * iIntros (?) "?". iApply bi_mono1_pers_mono; last done.
+        iModIntro. iIntros (a) "Hwp1". iNext. iMod "Hwp1". iModIntro.
+        by iApply "Hinner".
+      * iIntros (a) "Hwp1". iNext. by iApply "Hinner".
   Qed.
 
   Local Instance wpi_pre_monotone H :
-    BiMonoPred (λ wp_itree, uncurry (wpi_pre H (curry wp_itree))).
+    BiMonoPred (λ wpi, uncurry (wpi_pre H (curry wpi))).
   Proof.
     constructor.
     - iIntros (Π Ψ ??) "#Hinner". iIntros ([??]) "Hsim" => /=. iApply wpi_pre_mono; [|done].
@@ -113,121 +194,240 @@ Section wp_itree.
       apply wpi_pre_ne; eauto. move => ?????? /=. by apply: Hwp.
   Qed.
 
-  Definition wp_itree (H : iHandler Σ E) : itree E R → (R → iProp Σ) → iProp Σ :=
+  Definition wpi_opt (H : iHandler Σ EF) : itree E (option R) → (R → iProp Σ) → iProp Σ :=
     (* It is necessary to uncurry temporarily to get to the form
     [(A → iProp Σ) → (A → iProp Σ)] of which we can take the least fixpoint. *)
     curry (bi_least_fixpoint (λ wp_pre, uncurry (wpi_pre H (curry wp_pre)))).
+  Definition wpi (H : iHandler Σ EF) (t : itree E R) (Φ : R → iProp Σ) : iProp Σ :=
+    wpi_opt H (ITree.map Some t) Φ.
 
+  Global Instance wpi_opt_ne H n:
+    Proper ((eq_itree (=)) ==> ((=) ==> dist n) ==> dist n) (wpi_opt H).
+  Proof.
+    intros t1 t2 Ht Φ1 Φ2 HΦ. unfold wpi_opt. f_equiv; first done. intros ?. by apply HΦ. Qed.
   Global Instance wpi_ne H n:
-    Proper ((=) ==> ((=) ==> dist n) ==> dist n) (wp_itree H).
-  Proof. move => ?? -> ?? HΦ. unfold wp_itree. f_equiv. intros ?. by apply HΦ. Qed.
+    Proper ((eq_itree (=)) ==> ((=) ==> dist n) ==> dist n) (wpi H).
+  Proof.
+    intros t1 t2 Ht Φ1 Φ2 HΦ. unfold wpi. by repeat f_equiv.
+  Qed.
 End wp_itree.
 
-Notation "'WPi' t @ H {{ Φ } }" := (wp_itree H t%itree Φ)
+Notation "'WPi' t @ H {{ Φ } }" := (wpi H t%itree Φ)
   (at level 20, t, Φ at level 200, only parsing) : bi_scope.
-Notation "'WPi' t @ H {{ v , Q } }" := (wp_itree H t%itree (λ v, Q))
+Notation "'WPi' t @ H {{ v , Q } }" := (wpi H t%itree (λ v, Q))
   (at level 20, t, Q at level 200,
    format "'[hv' 'WPi'  t  '/' @  '[' H ']'  '/' {{  '[' v ,  '/' Q  ']' } } ']'") : bi_scope.
 
 Section wp_itree.
-  Context {Σ : gFunctors} {E : Type → Type} {H : iHandler Σ E}.
-  Context `{!invGS_gen HasNoLc Σ}.
+  Context {Σ : gFunctors} `{!EventFixpoint EF E} `{!invGS_gen HasNoLc Σ}.
+  Context {H : iHandler Σ EF}.
 
   Local Existing Instance wpi_pre_monotone.
-  Lemma wpi_unfold {R} (t : itree E R) Φ :
-    WPi t @ H {{ Φ }} ⊣⊢ wpi_pre H (wp_itree H) t Φ.
-  Proof. rewrite /wp_itree /curry. apply: least_fixpoint_unfold. Qed.
+  Lemma wpi_opt_unfold {R} (t : itree E (option R)) Φ :
+    wpi_opt H t Φ ⊣⊢ wpi_pre H (wpi_opt H) t Φ.
+  Proof. rewrite /wpi /curry. apply: least_fixpoint_unfold. Qed.
 
-  (* Induction principles for WPi. *)
-
-  Lemma wpi_strong_ind {R} (G: leibnizO (itree E R) -d> (leibnizO R -d> iPropO Σ) -d> iPropO Σ):
-    NonExpansive2 G →
-    ⊢ (□ ∀ t Φ, wpi_pre H (λ t' Ψ, G t' Ψ ∧ WPi t' @ H {{ Ψ }}) t Φ -∗ G t Φ)
-      -∗ ∀ t Φ, WPi t @ H {{ Φ }} -∗ G t Φ.
+  Global Instance wpi_opt_proper R :
+    Proper ((eqit (=) false false) ==> ((=) ==> (⊢)) ==> (⊢)) (wpi_opt (R:=R) H).
   Proof.
-    iIntros (Hne) "#HPre". iIntros (t Φ) "Hwp".
-    rewrite {2}/wp_itree {1}/curry.
-    iApply (least_fixpoint_ind _ (uncurry G) with "[] Hwp").
-    iIntros "!>" ([??]) "Hwp" => /=. by iApply "HPre".
+    move => t1 t2 Heqit Φ1 Φ2 HΦ. iIntros "Hwp".
+    iLöb as "IH" forall (t1 t2 Heqit).
+    rewrite /wpi !wpi_opt_unfold.
+    iMod "Hwp" as "[[%Ht >_]|[[%r [Hret Hr]]|[[%t' [% ?]]|(%A&%e&%k&%&Hwp)]]]".
+    - iLeft. iApply fupd_mask_intro; first done. iIntros "Hfupd".
+      iFrame. rewrite -Heqit. done.
+    - iModIntro. iRight. iLeft. iExists _. rewrite -Heqit. iFrame. by iApply HΦ.
+    - iModIntro. iRight. iRight. iLeft. iExists _. rewrite -Heqit. iSplit; first done.
+      iNext. by iApply "IH".
+    - iModIntro. iRight. iRight. iRight. iExists _, _, _. rewrite -Heqit. iSplit; first done.
+      iApply bi_mono1_mono; last done. iIntros (a) "Hwp". iNext. by iApply "IH".
   Qed.
-
-  Lemma wpi_ind {R} (G: leibnizO (itree E R) -d> (leibnizO R -d> iPropO Σ) -d> iPropO Σ):
-    NonExpansive2 G →
-    ⊢ (□ ∀ t Φ, wpi_pre H G t Φ -∗ G t Φ)
-      -∗ ∀ t Φ, WPi t @ H {{ Φ }} -∗ G t Φ.
-  Proof.
-    iIntros (Hne) "#HPre". iApply wpi_strong_ind. iIntros "!>" (t Φ) "Hwp".
-    iApply "HPre". iApply (wpi_pre_mono with "[] Hwp").
-    iIntros "!>" (??) "[? _]". by iFrame.
-  Qed.
-
   Global Instance wpi_proper R :
-    Proper ((eqit (=) false false) ==> (=) ==> (⊢)) (wp_itree (R:=R) H).
+      Proper ((eqit (=) false false) ==> (=) ==> (⊢)) (wpi (R:=R) H).
   Proof.
     move => t1 t2 Heqit ?? ->. iIntros "Hwp".
-    rewrite !wpi_unfold.
-    iMod "Hwp" as "[[%r [% Hwp]]|[[%t' [% Hwp]]|(%T&%e&%k&%&Hwp)]]";
-      iModIntro.
-    - iLeft. iExists _. iFrame. by rewrite -Heqit.
-    - iRight. iLeft. iExists _. iFrame. by rewrite -Heqit.
-    - iRight. iRight. iExists _, _, _. iFrame. by rewrite -Heqit.
+    rewrite /wpi.
+    iApply wpi_opt_proper; last done.
+    * by f_equiv.
+    * done.
   Qed.
 
   (** Rule of consequence. *)
+  Lemma wpi_opt_wand {R} (t : itree E (option R)) Φ Ψ:
+    (∀ r, Φ r -∗ Ψ r) -∗
+    wpi_opt H t Φ -∗
+    wpi_opt H t Ψ.
+  Proof.
+    iIntros "Hwand Hwp".
+    iLöb as "IH" forall (t).
+    rewrite /wpi !wpi_opt_unfold.
+    iMod "Hwp" as "[[%Ht >_]|[[%r [Hret Hr]]|[[%t' [% ?]]|(%A&%e&%k&%&Hwp)]]]".
+    - iLeft. iApply fupd_mask_intro; first done. iIntros "Hfupd". by iSplit.
+    - iModIntro. iRight. iLeft. iExists _. iSplit; [done|]. by iApply "Hwand".
+    - iModIntro. iRight. iRight. iLeft. iExists _. iSplit; [done|]. iModIntro.
+      by iApply ("IH" with "Hwand").
+    - iModIntro. iRight. iRight. iRight. iExists A, e, k. iSplit; first done.
+      iApply (bi_mono1_mono with "[Hwand] Hwp").
+      iIntros (a) "Hwp". iNext. by iApply ("IH" with "Hwand").
+  Qed.
   Lemma wpi_wand {R} (t : itree E R) Φ Ψ:
     (∀ r, Φ r -∗ Ψ r) -∗
     WPi t @ H {{ Φ }} -∗
     WPi t @ H {{ Ψ }}.
   Proof.
-    iIntros "Hwand Hwp".
-    pose (G := (λ t Ψ, ∀ Φ, (∀ r : R, Ψ r -∗ Φ r) -∗ WPi t @ H {{ Φ }})%I).
-    iAssert (∀ Φ, WPi t @ H {{ Φ }} -∗ G t Φ)%I as "Hgen"; last first.
-    { iApply ("Hgen" with "Hwp"). done. }
-    iIntros (?) "Hwp".
-    iApply (wpi_ind with "[] Hwp"). { solve_proper. }
-    iIntros "!>" (??) "Hwp". iIntros (?) "Hc".
-    rewrite wpi_unfold.
-    iMod "Hwp" as "[[%r [% Hwp]]|[[%t' [% Hwp]]|(%T&%e&%k&%&Hwp)]]"; iModIntro.
-    - iLeft. iExists _. iSplit; [done|]. by iApply "Hc".
-    - iRight. iLeft. iExists _. iSplit; [done|]. iModIntro. by iApply "Hwp".
-    - iRight. iRight. iExists _, _, _. iSplit; [done|].
-      iApply (bi_mono1_mono with "[Hc] Hwp"). iIntros (?) "Hwp". by iApply "Hwp".
+    rewrite /wpi. iApply wpi_opt_wand.
+  Qed.
+
+  Lemma map_ret_inv {R R'} (t : itree E R) (f : R → R') x :
+    ITree.map f t ≅ Ret x → ∃ y, f y = x ∧ t ≅ Ret y.
+  Proof.
+    intros Heqit.
+    apply eqitree_inv_Ret_r in Heqit.
+    destruct (observe t) as [r|t'|e h] eqn:Heq;
+    rewrite /ITree.map /ITree.bind /ITree.subst in Heqit; cbv in Heqit;
+    rewrite /observe in Heq; rewrite Heq in Heqit.
+    - injection Heqit as Heqit. eexists. split; first done.
+      apply fold_eqitF with (ot1 := RetF r) (ot2 := observe (Ret r)).
+      * simpl. by apply EqRet.
+      * done.
+      * done.
+    - discriminate.
+    - discriminate.
+  Qed.
+
+  (* Independence of post-condition if all termination is safe termination. *)
+  Lemma safe_termination_independent_post {T R R'} (t : itree E T) (Φ : R → iProp Σ) (Ψ : R' → iProp Σ) :
+    wpi_opt H (ITree.map (const None) t) Φ -∗ wpi_opt H (ITree.map (const None) t) Ψ.
+  Proof.
+    iIntros "Hwp".
+    iLöb as "IH" forall (T t Φ Ψ).
+    rewrite !wpi_opt_unfold.
+    iMod "Hwp" as "[[%Ht >_]|[[%r [%Hret Hwp]]|[[%t' [%Heq Hwp]]|(%A&%e&%k'&%Heq&Hwp)]]]".
+    - iLeft. iApply fupd_mask_intro; first done. iIntros "Hfupd". iFrame. iPureIntro.
+      apply map_ret_inv in Ht as [tt [_ Ht]]. rewrite Ht map_ret. reflexivity.
+    - apply map_ret_inv in Hret as [_ [[=] _]].
+    - iModIntro. iRight. iRight. iLeft. iExists (ITree.map (const None) t').
+      iSplit.
+      * iPureIntro.
+        assert (Heq' : ITree.map (const (@None R')) (ITree.map (const (@None R)) t)
+                     ≅ ITree.map (const (@None R')) (Tau t')).
+        { by f_equiv. }
+        transitivity (ITree.map (const (@None R')) (ITree.map (const (@None R)) t)).
+        { rewrite map_map. by apply eqit_eq_map. }
+        transitivity (ITree.map (const (@None R')) (Tau t')); first done.
+        by rewrite map_tau.
+      * iNext. iApply "IH".
+        rewrite (_ : ITree.map (const None) t' ≅ t'); first done.
+        apply eqit_inv_Tau.
+        rewrite -Heq -map_tau -Heq map_map. by apply eqit_eq_map.
+    - iModIntro. iRight. iRight. iRight.
+      iExists A, e, (λ a, ITree.map (const None) (k' a)).
+      iSplit.
+      * iPureIntro.
+        assert (Heq' : ITree.map (const (@None R')) (ITree.map (const (@None R)) t)
+                     ≅ ITree.map (const (@None R')) (Vis e k')).
+        { by f_equiv. }
+        transitivity (ITree.map (const (@None R')) (ITree.map (const (@None R)) t)).
+        { rewrite map_map. by apply eqit_eq_map. }
+        transitivity (ITree.map (const (@None R')) (Vis e k')); first done.
+        rewrite /ITree.map bind_vis. apply eqit_Vis. reflexivity.
+      * iApply bi_mono1_mono_l; [|iApply (bi_mono1_mono with "[] Hwp")].
+        + iIntros (Q) "Hwp". iApply bi_mono1_pers_mono; last done. iModIntro.
+          iIntros (t') "Hwp". iNext. iMod "Hwp". iModIntro. by iApply "IH".
+        + iIntros (a) "Hwp". iNext.
+          rewrite {1}(_ : k' a ≅ (ITree.map (const None) (k' a))). { by iApply "IH". }
+          generalize a.
+          (* Assumes UIP according to ITree documentation. *)
+          apply eqit_inv_Vis with (e := e).
+          transitivity ((ITree.map (const (@None R))) t); first done.
+          transitivity ((ITree.map (const (@None R))) ((ITree.map (const (@None R))) t)).
+          { rewrite map_map. by apply eqit_map with (RR:=(=)). }
+          transitivity (((ITree.map (const (@None R))) (Vis e k'))); first by f_equiv.
+          rewrite /ITree.map -bind_vis //.
+  Qed.
+
+  Lemma wpi_opt_always_None {R R'} Φ (t : itree E (option R)) :
+    (wpi_opt H t (const (|={∅,⊤}=> True))) -∗
+    (wpi_opt H (ITree.map (const (@None R')) t) Φ).
+  Proof.
+    iIntros "Hwp". iLöb as "IH" forall (R R' Φ t). rewrite /wpi !wpi_opt_unfold.
+    iMod "Hwp" as "[[%Ht >_]|[[%r [%Hret Hwp]]|[[%t' [%Heq Hwp]]|(%A&%e&%k'&%Heq&Hwp)]]]".
+    - iLeft. iApply fupd_mask_intro; first done. iIntros "Hfupd". iFrame. rewrite Ht map_ret //.
+    - simpl. iLeft. iModIntro. iFrame. rewrite Hret map_ret //.
+    - iModIntro. iRight. iRight. iLeft. iExists (ITree.map (const None) t').
+      iSplit.
+      * iPureIntro. rewrite Heq map_tau //.
+      * by iApply "IH".
+    - iRight. iRight. iRight.
+      iModIntro. iExists _, _, _. iSplit. { iPureIntro. rewrite Heq /ITree.map bind_vis //. }
+      iApply bi_mono1_mono_l; [|iApply (bi_mono1_mono with "[] Hwp")].
+      * iIntros (Q) "Hwp". iApply bi_mono1_pers_mono; last done.
+        iModIntro. iIntros (t') "Hwp". iNext. iMod "Hwp". iModIntro.
+        by iApply safe_termination_independent_post.
+      * iIntros (a) "Hwp". iNext. by iApply "IH".
+  Qed.
+
+  Lemma wpi_wpi_opt_always_None {R R'} Φ (t : itree E R) :
+    (WPi t @ H {{ const (|={∅,⊤}=> True) }}) -∗
+    (wpi_opt H (ITree.map (const (@None R')) t) Φ).
+  Proof.
+    rewrite /wpi.
+    rewrite (_ : (ITree.map (const None) t) ≅ (ITree.map (const None) (ITree.map Some t))).
+    - iApply wpi_opt_always_None.
+    - rewrite map_map. by apply eqit_map with (RR:=(=)).
   Qed.
 
   (* Monadic rules. *)
 
+  Lemma wpi_opt_bind {R R'} (t : itree E (option R)) (k : R → itree E (option R')) Φ :
+    wpi_opt H t (λ r, wpi_opt H (k r) Φ) -∗
+    wpi_opt H (ITree.bind t (λ r, match r with
+                                | None => Ret None
+                                | Some r => k r
+                                end)) Φ.
+  Proof.
+    iIntros "Hwp".
+    iLöb as "IH" forall (t Φ).
+    rewrite /wpi !wpi_opt_unfold.
+    iMod "Hwp" as "[[%Ht >_]|[[%r [%Hret Hwp]]|[[%t' [%Heq ?]]|(%A&%e&%k'&%Heq&Hwp)]]]".
+    - iLeft. iApply fupd_mask_intro; first done. iIntros "Hfupd". iFrame. iPureIntro.
+      rewrite Ht bind_ret_l //.
+    - rewrite wpi_opt_unfold.
+      iMod "Hwp" as "[[%Ht >_]|[[%r' [%Hret' Hwp]]|[[%t' [% ?]]|(%A&%e&%k'&%&Hwp)]]]".
+      * iLeft. iApply fupd_mask_intro; first done. iIntros "Hfupd". iFrame. iPureIntro.
+        rewrite Hret bind_ret_l //.
+      * iModIntro. iRight. iLeft. iExists _. iSplit; [iPureIntro|done]. by rewrite Hret bind_ret_l.
+      * iModIntro. iRight. iRight. iLeft. iExists _. iSplit; [iPureIntro|done].
+        by rewrite Hret bind_ret_l.
+      * iModIntro. iRight. iRight. iRight. iExists _,_,_. iSplit; [iPureIntro|done].
+        by rewrite Hret bind_ret_l.
+    - iModIntro. iRight. iRight. iLeft. iExists _. iSplit. { iPureIntro. by rewrite Heq bind_tau. }
+      iModIntro. by iApply "IH".
+    - iModIntro. iRight. iRight. iRight. iExists _, _, _. iSplit.
+      { iPureIntro. by rewrite Heq bind_vis. }
+      iApply bi_mono1_mono_l; [|iApply (bi_mono1_mono with "[] Hwp")].
+      * iIntros (Q) "Hwp". iApply bi_mono1_pers_mono; last done. iModIntro.
+        iIntros (a) "Hwp". iNext. iMod "Hwp". iModIntro.
+        by iApply safe_termination_independent_post.
+      * iIntros (a) "Hwp". iNext. by iApply "IH".
+  Qed.
   Lemma wpi_bind {R T} (t : itree E T) (k : T → itree E R) Φ :
     WPi t @ H {{ r, WPi (k r) @ H {{ Φ }} }} -∗
     WPi (ITree.bind t k) @ H {{ Φ }}.
   Proof.
+    rewrite /wpi.
     iIntros "Hwp".
-    pose (G := (λ t Ψ, ∀ Φ, (∀ r, Ψ r -∗ WPi k r @ H {{ Φ }}) -∗ WPi ITree.bind t k @ H {{ Φ }})%I).
-    iAssert (∀ Φ, WPi t @ H {{ Φ }} -∗ G t Φ)%I as "Hgen"; last first.
-    { iApply ("Hgen" with "Hwp"). iIntros (?) "?". done. }
-    iIntros (?) "Hwp".
-    iApply (wpi_ind with "[] Hwp"). { solve_proper. }
-    iIntros "!>" (??) "Hwp". iIntros (?) "Hc".
-    rewrite wpi_unfold.
-    iMod "Hwp" as "[[%r [%Heq Hwp]]|[[%t' [%Heq Hwp]]|(%X&%e&%j&%Heq&Hwp)]]".
-    - iDestruct ("Hc" with "[$]") as "Hc". rewrite wpi_unfold.
-      iMod "Hc" as "[[%r' [%Heq' Hwp]]|[[%t' [% Hwp]]|(%X&%e&%j&%&Hwp)]]"; iModIntro.
-      + iLeft. iExists _. iSplit; [iPureIntro|done]. by rewrite Heq bind_ret_l.
-      + iRight. iLeft. iExists _. iSplit; [iPureIntro|done]. by rewrite Heq bind_ret_l.
-      + iRight. iRight. iExists _,_,_. iSplit; [iPureIntro|done].
-        by rewrite Heq bind_ret_l.
-    - iModIntro. iRight. iLeft. iExists _. iSplit. { iPureIntro. by rewrite Heq bind_tau. }
-      iModIntro. by iApply "Hwp".
-    - iModIntro. iRight. iRight. iExists _, _, _. iSplit.
-      { iPureIntro. by rewrite Heq bind_vis. }
-      iApply (bi_mono1_mono with "[Hc] Hwp"). iIntros (?) "Hwp". by iApply "Hwp".
+    rewrite (_ : ITree.map Some (ITree.bind t k) ≅ _).
+    - by iApply wpi_opt_bind.
+    - rewrite bind_map /ITree.map bind_bind //.
   Qed.
 
   Lemma wpi_ret {R} Φ (r : R):
     Φ r -∗
     WPi Ret r @ H {{ Φ }}.
   Proof.
-    iIntros "HΦ". rewrite wpi_unfold. iIntros "!>".
-    iLeft. iExists _. by iFrame.
+    iIntros "HΦ". rewrite /wpi wpi_opt_unfold. iIntros "!>".
+    iRight. iLeft. iExists _. iFrame. rewrite map_ret //.
   Qed.
 
   (* Other basic cases. *)
@@ -236,17 +436,28 @@ Section wp_itree.
     ▷ WPi t @ H {{ Φ }} -∗
     WPi Tau t @ H {{ Φ }}.
   Proof.
-    iIntros "Hwp". iEval (rewrite wpi_unfold). iIntros "!>".
-    iRight. iLeft. iExists _. iSplit; [done|]. by iModIntro.
+    iIntros "Hwp". iEval (rewrite /wpi wpi_opt_unfold). iIntros "!>".
+    iRight. iRight. iLeft. iExists _. iSplit.
+    - by rewrite map_tau.
+    - done.
   Qed.
 
-  Lemma wpi_vis {R} Φ T e (k : T → itree E R):
-    H T e (λ r, WPi k r @ H {{ Φ }}) -∗
+  Lemma wpi_vis {R} Φ A (e : E A) (k : A → itree E R):
+    H E A (subevent A e) (λ r, ▷ WPi k r @ H {{ Φ }}) (λ t, ▷ |={⊤, ∅}=> WPi t @ H {{ const (|={∅, ⊤}=> True) }}) -∗
     WPi (Vis e k) @ H {{ Φ }}.
   Proof.
-    iIntros "Hwp". iEval (rewrite wpi_unfold). iIntros "!>".
-    iRight. iRight. iExists _, _, _. iSplit; [done|].
-    iApply (bi_mono1_intro with "[] Hwp"). by iIntros (?) "?".
+    iIntros "Hwp". rewrite /wpi !wpi_opt_unfold. iIntros "!>".
+    iRight. iRight. iRight. iExists _, _, _. iSplit.
+    * iPureIntro. rewrite /ITree.map bind_vis //.
+    * iApply (bi_mono1_mono with "[] [Hwp]"); first shelve.
+      iApply (bi_mono1_intro with "[] [Hwp]"). { iIntros (a) "Hgoal". done. }
+      iApply (bi_mono1_pers_mono with "[] [Hwp]"); first shelve.
+      iApply (bi_mono1_pers_intro with "[] [Hwp]"). { iModIntro. iIntros (a) "Hgoal". done. }
+      done.
+      Unshelve.
+      + by iIntros (a) "Hwp".
+      + iModIntro. iIntros (t) "Hwp". iNext. iMod "Hwp". iModIntro.
+        rewrite /ITree.map. by iApply wpi_wpi_opt_always_None.
   Qed.
 
   (* Derived rules. *)
@@ -268,12 +479,14 @@ Section wp_itree.
     iApply (wpi_wand with "[HP]"); last exact.
     eauto with iFrame.
   Qed.
+
 End wp_itree.
 
 Section translation.
-  Context {Σ : gFunctors} {E1 E2 : Type → Type} {f : E1 ~> itree E2}.
-  Context {H1 : iHandler Σ E1} {H2 : iHandler Σ E2}.
-  Context `{!invGS_gen HasNoLc Σ}.
+  Context {Σ : gFunctors} `{!invGS_gen HasNoLc Σ}.
+  Context `{!EventFixpoint EF1 E1} `{!EventFixpoint EF2 E2}.
+  Context {H1 : iHandler Σ EF1} {H2 : iHandler Σ EF2}.
+  Context {f : E1 ~> itree E2}.
 
   (* Translation lemma. *)
 
@@ -284,13 +497,9 @@ Section translation.
   interp f t @ H1 {{ Φ }}] for itrees [t]. The following statement gives you
   sufficient conditions for when one implies the other. *)
   Lemma wp_translation {R} :
-    □ (∀ A (e : E1 A) Q Q', (∀ v, Q v -∗ Q' v) -∗ H1 A e Q -∗ H1 A e Q') -∗
-    □ (∀ A (e : E1 A) ψ, H1 A e ψ -∗ WPi (f A e) @ H2 {{ v, ψ v }}) -∗
+    □ (∀ A e Φ s, (∀ v, Φ v -∗ Φ v) -∗ H1 E1 A e Φ s -∗ H1 E1 A e Φ s) -∗
+    □ (∀ A (e : E1 A) ψ, H1 E1 A e ψ -∗ WPi (f A e) @ H2 {{ v, ψ v }}) -∗
     ∀ (t : itree E1 R) Φ, WPi t @ H1 {{ Φ }} -∗ WPi (interp f t) @ H2 {{ Φ }}.
-  (** One could hope for a converse statement, but unfortunately the proof
-  makes use of [wpi_bind] which is a one-way implication (because it in turn
-  makes use of [wpi_ind]). If [wpi_bind] was instead an equivalence, it
-  would in fact be possible to prove a converse statement. *)
   Proof.
     iIntros "#Hmon #HH". iApply wpi_ind.
     - intros n t1 t2 Heqnt φ1 φ2 Heqnφ. apply wpi_ne.
