src/event.v
@@ -1,0 +1,25 @@
+From stdpp Require Import prelude.
+From ITree Require Import ITree.
+
+Class SubeventF (EF1 EF2 : (Type → Type) → Type → Type) :=
+  incl : ∀ preE, EF1 preE ~> EF2 preE.
+
+Notation "E --< F" := (SubeventF E F)
+  (at level 92, left associativity) : type_scope.
+
+Definition subeventF {EF1 EF2 : (Type → Type) → Type → Type} {preE : Type → Type} `{EF1 --< EF2}
+  : EF1 preE ~> EF2 preE := incl preE.
+
+Global Instance subeventF_id EF : SubeventF EF EF := { incl := λ preE A, id }.
+
+Global Instance subeventF_subevent E `{!SubeventF EF1 EF2} : Subevent (EF1 E) (EF2 E) :=
+  { resum := incl E }.
+
+Class EventFixpoint (EF : (Type → Type) → Type → Type) (E : Type → Type) :=
+  eq_fix : E = EF E.
+
+Import EqNotations.
+Global Instance subevent_fixpoint `{!EventFixpoint EF E} : Subevent E (EF E) :=
+  { resum := λ A e, rew [λ T, T A] eq_fix in e }.
+Global Instance subevent_fixpoint' `{!EventFixpoint EF E} : Subevent (EF E) E :=
+  { resum := λ A e, rew [λ T, T A] (eq_sym eq_fix) in e }.
